



Is it possible to hang the purse from two pegs so that it stays up, but will fall if either peg is removed?

(none of the above work!)

Plan: Matrix algebra

Basic building block of matrix multiplication  
is row  $\times$  column = number

$$a \cdot x = [a_1, a_2, \dots, a_n] \cdot \begin{bmatrix} x_1 \\ \vdots \\ x_n \end{bmatrix} = a_1 x_1 + a_2 x_2 + \dots + a_n x_n$$

$x_i$ 's = variables.

$$a \cdot v = [a_1, \dots, a_n] \begin{bmatrix} v_1 \\ \vdots \\ v_n \end{bmatrix} = a_1 v_1 + \dots + a_n v_n$$

$v_i$ 's = #'s

Given a system :

$$a_{11}x_1 + \dots + a_{1n}x_n = b_1$$

$$a_{21}x_1 + \dots + a_{2n}x_n = b_2$$

$\vdots$

$$a_{m1}x_1 + \dots + a_{mn}x_n = b_m$$

we "stack the notation"

$$\begin{bmatrix} a_{11} & a_{12} & \dots & a_{1n} \\ a_{21} & \dots & \dots & a_{2n} \\ \vdots & & & \vdots \\ a_{m1} & \dots & \dots & a_{mn} \end{bmatrix} \begin{bmatrix} x_1 \\ \vdots \\ x_n \end{bmatrix} = \begin{bmatrix} b_1 \\ b_2 \\ \vdots \\ b_m \end{bmatrix}$$

$$(a_{21} \dots a_{2n}) \begin{bmatrix} x_1 \\ \vdots \\ x_n \end{bmatrix} = b_2$$

In general: if  $A = \begin{bmatrix} a_{11} & \dots & a_{1n} \\ \vdots & & \vdots \\ a_{m1} & \dots & a_{mn} \end{bmatrix}$   $C = \begin{bmatrix} c_{11} & \dots & c_{1r} \\ \vdots & & \vdots \\ c_{m1} & \dots & c_{mr} \end{bmatrix}$

$A \cdot C$  = matrix w/  $i, j$  entry =  $i$ th row of  $A$   
 $j$ th row of  $C$

Idea: rows on left  
columns on right

$$A = \left[ \begin{array}{c} \hline A_1 \\ \hline A_2 \\ \hline \vdots \\ \hline A_m \end{array} \right]$$

$$B = \left[ \begin{array}{c|c|c} B_1 & \dots & B_r \end{array} \right]$$

$$A \cdot B = \begin{bmatrix} A_1 \cdot B_1 & A_1 \cdot B_2 & A_1 \cdot B_3 & \dots & A_1 \cdot B_r \\ \vdots & \vdots & \vdots & & \vdots \\ A_m \cdot B_1 & - & - & - & A_m \cdot B_r \end{bmatrix}$$

note: for this to make sense, length of rows in A  
= length of columns in B

$$(m \times n) \cdot (n \times r) = (m \times r)$$

Note: dot product has same concept properties, that the  
matrix product inherits:

$$A \cdot (B_1 + B_2) = A \cdot B_1 + A \cdot B_2$$

$$(A_1 + A_2) \cdot B = A_1 \cdot B + A_2 \cdot B$$

So here: addition of matrices is inherited from addition  
of vectors

$$A = \begin{bmatrix} A_1 \\ A_2 \\ \vdots \\ A_m \end{bmatrix} \quad B = \begin{bmatrix} B_1 \\ \vdots \\ B_n \end{bmatrix}$$

$$A + B = \begin{bmatrix} A_1 + B_1 \\ \vdots \\ A_m + B_m \end{bmatrix}$$

or - slice vertically - or just add each entry.

## Quick matrix theory primer

Solve  $Ax=b$  inhom. system of eqns.  
 $x, b = \text{column vectors}$   
 $(A\vec{x} = \vec{b})$

Prop: if  $v$  is any soln to  $Ax=b$  (i.e.  $Av=b$ )  
and  $w$  is any soln to  $Ax=0$  then  $v+w$  is  
a soln to  $Ax=b$

and conversely, every soln to  $Ax=b$  has the form  
 $x=v+w$  where  $w$  is a soln to  $Ax=0$ .

why? if  $Av=b$  &  $Aw=0$

$$b = b+0 = Av + Aw = A(v+w)$$

$v+w$  is a soln to  $Ax=b$

conversely: if  $v'$  is any other soln to  $Ax=b$

$$\text{then } A(v'-v) = Av' - Av = b - b = 0$$

set  $w = v' - v$  is a soln to  $Ax=0$

$$\text{and } v' = v + w \quad \checkmark$$

Remarkably matrix multiplication is associative too  
 $(AB)C = A(BC)$

# Row operations

when we write  $Tx = b$   $T$  an  $m \times n$  matrix

$T$  gives rule for taking a column w/  $n$  entries  
to a column w/  $m$  entries.

$$T: \mathbb{R}^n \rightarrow \mathbb{R}^m$$

$$T = \begin{pmatrix} a_{11} & a_{12} & \dots & a_{1n} \\ \vdots & \vdots & \ddots & \vdots \\ a_{m1} & \dots & \dots & a_{mn} \end{pmatrix}$$

$$\begin{matrix} A_1 \\ \vdots \\ A_m \end{matrix} \begin{pmatrix} a_{11} & a_{12} & \dots & a_{1n} \\ \vdots & \vdots & \ddots & \vdots \\ a_{m1} & \dots & \dots & a_{mn} \end{pmatrix} \begin{pmatrix} v_1 \\ \vdots \\ v_n \end{pmatrix} = \begin{pmatrix} A_1 \cdot \vec{v} \\ \vdots \\ A_m \cdot \vec{v} \end{pmatrix}$$

ex:  $\begin{bmatrix} v_1 \\ v_2 \\ \vdots \\ v_n \end{bmatrix} \mapsto \begin{bmatrix} v_2 \\ v_1 \\ v_3 \\ \vdots \\ v_n \end{bmatrix}$  this is a function.  
is it given by a matrix?

$$\begin{bmatrix} v_1 \\ v_2 \end{bmatrix} \mapsto \begin{bmatrix} v_2 \\ v_1 \end{bmatrix}$$

$$\begin{bmatrix} 0 & 1 \\ 1 & 0 \end{bmatrix} \begin{bmatrix} v_1 \\ v_2 \end{bmatrix} = \begin{bmatrix} v_2 \\ v_1 \end{bmatrix}$$

$$0 + v_2 = v_2$$

$$v_1 + 0 = v_1$$

$$\begin{bmatrix} 0 & 1 & 0 & \dots \\ 1 & 0 & \dots & \dots \\ 0 & 0 & 1 & \dots \\ \vdots & \vdots & \vdots & \ddots \end{bmatrix}$$

$$\begin{bmatrix} 0 & 1 & & 0 \\ 1 & 0 & & 0 \\ & & \ddots & \\ 0 & & & 1 \end{bmatrix} \begin{bmatrix} -\frac{R_1}{R_2} \\ \vdots \\ R_n \end{bmatrix}$$

$$\begin{bmatrix} v_1 \\ \vdots \\ v_n \end{bmatrix} \xrightarrow{T} \begin{bmatrix} \lambda v_1 \\ v_2 \\ \vdots \\ v_n \end{bmatrix}$$

$$\begin{aligned} \lambda v_1 &= \lambda v_1 + 0v_2 + \dots \\ v_2 &= 0v_1 + 1v_2 + 0v_3 + \dots \\ v_3 &= 0v_1 + 0v_2 + 1v_3 + \dots \\ &\vdots \\ v_n &= \end{aligned}$$

$$\begin{bmatrix} \lambda & 1 & & 0 \\ & 1 & & 0 \\ & & \ddots & \\ 0 & & & 1 \end{bmatrix} \begin{bmatrix} -\frac{R_1}{R_2} \\ \vdots \\ R_n \end{bmatrix} = \begin{bmatrix} \lambda R_1 \\ \frac{R_1}{R_2} \\ \vdots \\ R_n \end{bmatrix}$$

$$\begin{bmatrix} 1 & 0 \\ \lambda & 1 \end{bmatrix} \begin{bmatrix} v_1 \\ v_2 \end{bmatrix} = \begin{bmatrix} v_1 \\ \lambda v_1 + v_2 \end{bmatrix} = \begin{bmatrix} 1v_1 + 0v_2 \\ \lambda v_1 + 1v_2 \end{bmatrix}$$

$$\begin{bmatrix} 1 & 0 \\ \lambda & 1 & & \\ & 1 & & \\ & & \ddots & \\ & & & 1 \end{bmatrix} \begin{bmatrix} -\frac{R_1}{R_2} \\ \vdots \\ R_n \end{bmatrix} = \begin{bmatrix} -\frac{R_1}{R_2} \\ \lambda R_1 + R_2 \\ \vdots \\ R_n \end{bmatrix}$$

Punchline: if  $A = \begin{pmatrix} a_{11} & \dots \\ \vdots & \end{pmatrix}$  coeffs of system of  
(nr eqns)

$$Ax = b$$

then for each elementary row operation

- swap rows (I)
- mult. row by scalar (II)
- add mult. of one row to another (III)

there's a (very simple) matrix  $E$  s.t.

$E \cdot A$  gives the transformed set of eqns.

correspond "elementary matrices" - of types I, II, III  
corresp. to these.

ex:

$$2x + 3y = 5$$

$$x - y = 1$$

$$\begin{bmatrix} 2 & 3 \\ 1 & -1 \end{bmatrix} \begin{bmatrix} x \\ y \end{bmatrix} = \begin{bmatrix} 5 \\ 1 \end{bmatrix}$$

$\begin{matrix} \text{"} & \text{"} & \text{"} \\ A & v & b \end{matrix}$

[p. 17]

$$\begin{aligned}
 \begin{bmatrix} 2 & 3 \\ 1 & -1 \end{bmatrix} &\xrightarrow{E_1 = L^{-1}} \begin{bmatrix} 1 & -1 \\ 2 & 3 \end{bmatrix} \xrightarrow{-2} \begin{bmatrix} 1 & -1 \\ 0 & 5 \end{bmatrix} = E_2 \\
 &\downarrow \begin{bmatrix} 1 & 0 \\ -2 & 1 \end{bmatrix} \\
 \begin{bmatrix} 1 & -1 \\ 0 & 5 \end{bmatrix} &\cdot \frac{1}{5} \rightarrow \begin{bmatrix} 1 & -1 \\ 0 & 1 \end{bmatrix} = E_3 \\
 &\downarrow \begin{bmatrix} 1 & 0 \\ 0 & 1 \end{bmatrix} \\
 \begin{bmatrix} 1 & 0 \\ 0 & 1 \end{bmatrix} &= E_4
 \end{aligned}$$

$$\underbrace{E_4 E_3 E_2 E_1}_E A = \begin{bmatrix} 1 & 0 \\ 0 & 1 \end{bmatrix}$$

$$Av = b$$

$$r = \underbrace{E}_A A v = E b$$

$$x_1 + 0x_2 = x_1$$

$$0 + 1x_2 = x_2$$

$E \leftrightarrow$  "inverse of  $A$ "  
 $\begin{bmatrix} 1 & 0 \\ 0 & 1 \end{bmatrix} \leftrightarrow$  identity.